Spectral Element Method Formulation
===================================

This chapter is for documenting the theoretical aspect of the solver and
associated routines. One can refer to the equations and the
corresponding code to be clear about the implementations.

Seismic Wave Equation: FEM Solver
---------------------------------

Weak form and element matrices
~~~~~~~~~~~~~~~~~~~~~~~~~~~~~~

We are solving the seismic wave equation in 2D:

.. math::

   \begin{aligned}
   \rho \ddot{u}_{\rm{i}} = \partial_{\rm{j}} \tau_{\rm{ij}} + f_{\rm{i}}
   \end{aligned}

The above equation is in component form where the subscript i denotes
the component of :math:`\vec{u}`. :math:`\tau_{\rm{ij}}` is the second
order stress tensor and :math:`\vec{f}` denotes the external force
distribution. :math:`\tau_{\rm{ij}}` is expressed as:

.. math:: \tau_{\rm{ij}} = \lambda \delta_{\rm{ij}} e_{\rm{kk}} + 2 \mu e_{\rm{ij}}

and,

.. math:: e_{\rm{ij}} = \frac{1}{2}(\partial_{\rm{i}}u_{\rm{j}} + \partial_{\rm{j}}u_{\rm{i}})

Therefore, the wave equation reads as:

.. math::

   \begin{aligned}
   \rho \ddot{u}_{\rm{i}} = \partial_{\rm{j}}\bigg(\frac{\lambda \delta_{\rm{ij}}}{2}(\partial_{\rm{k}}u_{\rm{k}} + \partial_{\rm{k}}u_{\rm{k}})\bigg) + \partial_{\rm{j}}\bigg(\mu (\partial_{\rm{i}}u_{\rm{j}} + \partial_{\rm{j}}u_{\rm{i}}) \bigg) + f_{\rm{i}}\end{aligned}

For starting off, we consider constant :math:`\lambda` and :math:`\mu`.
So, we assume homogeneous and isotropic medium properties.

.. math::

   \begin{aligned}
   \rho \ddot{u}_{\rm{i}} = \lambda \partial_{\rm{i}}(\partial_{\rm{k}} u_{\rm{k}}) + \mu(\partial_{\rm{i}}(\partial_{\rm{j}}u_{\rm{j}}) + \partial_{\rm{j}}^2 u_{\rm{i}})\end{aligned}

Hereafter, we switch to the weak formulation and multiply
:math:`N_{\rm{l}}`, the :math:`l`-th shape function throughout the
equation and integrate over the area element :math:`dxdy`. We expand the
displacement :math:`\vec{u}` in terms of the components
:math:`u_{\rm{i}}(x,y) = \sum_{m=1}^{nip} u_{\rm{i}}^{\rm{m}}(x,y) N_{\rm{m}}(x,y)`,
where :math:`nip` is the total number of GLL points per element where
integration has to be carried out. Therefore, the term on the left hand
side becomes:

.. math::

   \begin{aligned}
   &=& \int N_l(x,y) \rho(x,y) \ddot{u}_{\rm{i}}(x,y)dxdy \\
   &=& \int_{-1}^{1} N_l(\xi,\eta) \rho(\xi,\eta) \sum_{m=1}^{nip} \ddot{u}_{\rm{i}}^{\rm{m}} N_{\rm{m}}(\xi,\eta) \mathcal{J}(\xi,\eta) d\xi d\eta \\
   &=& \sum_{k=1}^{nip} N_l(\xi_{\rm{k}},\eta_{\rm{k}}) \rho(\xi_{\rm{k}},\eta_{\rm{k}}) \sum_{m=1}^{nip} \ddot{u}_{\rm{i}}^{\rm{m}} N_{\rm{m}}(\xi_{\rm{k}},\eta_{\rm{k}}) \mathcal{J}(\xi_{\rm{k}},\eta_{\rm{k}}) W_{\rm{k}},\end{aligned}

where :math:`W_{\rm{k}} = w_{\rm{k1}} w_{\rm{k2}}`, the product of the
weights of the constitutive lagrange polynomials at those GLL points.
:math:`\mathcal{J}` is the determinant of the Jacobian for transforming
the integral variables from global to local coordinates. So, we sum over
all the GLL points in an element with adequate weights to perform the 2D
integral. However, the shape functions
:math:`N_{\rm{m}}(\xi_{\rm{k}},\eta_{\rm{k}}) = \delta_{\rm{mk}}` and
hence the remaining summation can be expressed as a product of a
diagonal mass matrix and a column vector :math:`u_{\rm{i}}`.

.. math:: \sum_{k=1}^{nip} \rho(\xi_{\rm{k}},\eta_{\rm{k}}) \mathcal{J}(\xi_{\rm{k}},\eta_{\rm{k}}) W_{\rm{k}} \ddot{u}_{\rm{i}}^{\rm{k}}

Hence we are finally left with the local mass matrix:
:math:`\rho(\xi_{\rm{k}},\eta_{\rm{k}}) \mathcal{J}(\xi_{\rm{k}},\eta_{\rm{k}}) W_{\rm{k}}`,
where :math:`k` is the GLL point number for an element. These will form
the diagonal elements of out matrix for each element.

The vectorial representation of the second term in 3D looks like the
following:

.. math::

   \begin{aligned}
   \int_V N_l \nabla \cdot \mathbf{\tau} dV\end{aligned}

Using Gaussâ€™ theorem and assuming a stress free boundary condition such
that :math:`\mathbf{\tau}\cdot \mathbf{\hat{\mathbf{n}}} = 0,` where
:math:`\mathbf{\hat{\mathbf{n}}}` is the normal to the boundary surface.
So, we are left with:

.. math::

   \begin{aligned}
   \int_V N_l \nabla \cdot \mathbf{\tau} dV = -\int_V \nabla N_l \cdot \mathbf{\tau}dV\end{aligned}

In case of 2D, writing in a component form yields the equations:

.. math::

   \begin{aligned}
   &=& -\int \partial_j N_l \tau_{ij} dxdy \\
   &=& -\int \partial_j N_l(x,y) \lambda(x,y) \delta_{ij} \partial_r u_r dxdy \nonumber \\ &-& \int \partial_j N_l(x,y) \mu(x,y)(\partial_i u_j + \partial_j u_i)dxdy\end{aligned}

Let the first term be A:

.. math::

   \begin{aligned}
   &=& -\int \partial_j N_l(x,y) \lambda(x,y) \delta_{ij} \partial_r \sum_m N_m(x,y) u_r^m dxdy\end{aligned}

While the second term can be split into B and C respectively:

.. math::

   \begin{aligned}
   &-& \int \partial_j N_l(x,y) \mu(x,y) \partial_i \sum_m N_m(x,y) u_j^m \nonumber \\ &-&  \int \partial_j N_l \mu(x,y) \partial_j \sum_m N_m(x,y) u_j^m dxdy\end{aligned}

Now, we can convert the global coordinates (x,y) to local coordinate
(:math:`\xi,\eta`) using the Jacobian :math:`\mathcal{J(\xi,\eta)}` and
use the quadrature to further simplifiy the integral into:

.. math::

   \begin{aligned}
   A &= -\int_{-1}^{1} \partial_i N_l(\xi,\eta) \left. \frac{\partial \mathbf{\xi}}{\partial \mathbf{x}} \right|_{\xi,\eta} \lambda(\xi,\eta) \sum_m \partial_r N_m(\xi,\eta) \left. \frac{\partial \mathbf{\xi}}{\partial \mathbf{x}} \right|_{\xi,\eta} u_r^m \left| \mathcal{J}(\xi,\eta) \right|  d\eta d\xi \\
   &= -\sum_{k=1}^{nip} \partial_i N_l(\xi_k,\eta_k)\left. \frac{\partial \mathbf{\xi}}{\partial \mathbf{x}} \right|_{\xi_k,\eta_k} \lambda(\xi_k,\eta_k) \sum_m \partial_r N_m(\xi_k,\eta_k)\left. \frac{\partial \mathbf{\xi}}{\partial \mathbf{x}} \right|_{\xi_k,\eta_k} u_r^m \left| \mathcal{J} (\xi_k,\eta_k)\right| W_k \nonumber \\
   &= -\sum_{m=1}^{nip} u_{\mathbf{r}}^m \sum_{k=1}^{nip} \lambda(\xi_k,\eta_k) \partial_i N_l(\xi_k,\eta_k)\left. \frac{\partial \mathbf{\xi}}{\partial \mathbf{x}} \right|_{\xi_k,\eta_k}  \partial_{\mathbf{r}} N_m(\xi_k,\eta_k) \left. \frac{\partial \mathbf{\xi}}{\partial \mathbf{x}} \right|_{\xi_k,\eta_k}  \left| \mathcal{J}(\xi_k,\eta_k) \right| W_k \nonumber\\
   \end{aligned}

The bars around the :math:`\mathcal{J}` denote the determinant. The 
bold subscript is to remind ourselves that the index needs to be
summed over for all the components (:math:`x` and :math:`y` in 2D and
:math:`x,y` and :math:`z` in 3D). Similarly,

.. math::

   \begin{aligned}
   B &= - \int_{-1}^{1} \partial_j N_l(\xi,\eta) \left. \frac{\partial \mathbf{\xi}}{\partial \mathbf{x}} \right|_{\xi,\eta} \mu(\xi,\eta) \sum_m \partial_i N_m(\xi,\eta)\left. \frac{\partial \mathbf{\xi}}{\partial \mathbf{x}} \right|_{\xi,\eta} u_j^m \left| \mathcal{J}(\xi_k,\eta_k) \right| d\xi d\eta \\
   &= -\sum_{k=1}^{nip} \partial_j N_l(\xi_k,\eta_k) \left. \frac{\partial \mathbf{\xi}}{\partial \mathbf{x}} \right|_{\xi_k,\eta_k} \mu(\xi_k,\eta_k) \sum_m \partial_i N_m(\xi_k,\eta_k)\left. \frac{\partial \mathbf{\xi}}{\partial \mathbf{x}} \right|_{\xi_k,\eta_k} u_j^m \left| \mathcal{J}(\xi_k,\eta_k) \right| W_k \nonumber \\ \\
   &= -\sum_{m=1}^{nip} u_{\mathbf{j}}^m \sum_{k=1}^{nip} \mu(\xi_k,\eta_k) \partial_{\mathbf{j}} N_l(\xi_k,\eta_k) \left. \frac{\partial \mathbf{\xi}}{\partial \mathbf{x}} \right|_{\xi_k,\eta_k} \partial_i N_m(\xi_k,\eta_k) \left. \frac{\partial \mathbf{\xi}}{\partial \mathbf{x}} \right|_{\xi_k,\eta_k}  \left| \mathcal{J}(\xi_k,\eta_k) \right| W_k \nonumber \\
   \end{aligned}

Finally,

.. math::

   \begin{aligned}
   C &= -\int_{-1}^{1} \partial_j N_l(\xi,\eta) \left. \frac{\partial \mathbf{\xi}}{\partial \mathbf{x}} \right|_{\xi,\eta} \mu(\xi,\eta) \sum_m \partial_j N_m(\xi,\eta)\left. \frac{\partial \mathbf{\xi}}{\partial \mathbf{x}} \right|_{\xi,\eta} u_i^m \left| \mathcal{J}(\xi_k,\eta_k) \right|(\xi,\eta) d\xi d\eta \\
   &= -\sum_{k=1}^{nip} \partial_j N_l(\xi_k,\eta_k)\left. \frac{\partial \mathbf{\xi}}{\partial \mathbf{x}} \right|_{\xi_k,\eta_k} \mu(\xi_k,\eta_k) \sum_m \partial_j N_m(\xi_k,\eta_k)\left. \frac{\partial \mathbf{\xi}}{\partial \mathbf{x}} \right|_{\xi_k,\eta_k} u_i^m \left| \mathcal{J}(\xi_k,\eta_k) \right|(\xi_k,\eta_k) W_k \nonumber\\ \\
   &= -\sum_{m=1}^{nip} u_i^m \sum_{k=1}^{nip} \mu(\xi_k,\eta_k) \partial_{\mathbf{j}} N_l(\xi_k,\eta_k)\left. \frac{\partial \mathbf{\xi}}{\partial \mathbf{x}} \right|_{\xi_k,\eta_k} \partial_{\mathbf{j}} N_m(\xi_k,\eta_k)\left. \frac{\partial \mathbf{\xi}}{\partial \mathbf{x}} \right|_{\xi_k,\eta_k} \left| \mathcal{J}(\xi_k,\eta_k) \right|(\xi_k,\eta_k) W_k \nonumber\\ 
   \end{aligned}


If we notice, the expression of A, B and C have free indices as
:math:`l` and :math:`i`. Here, :math:`i` denotes the component of
:math:`\vec{u}` that we are solving for and :math:`l` denotes the row
number of the column vector :math:`u_i`.

As of know this algorith is followed strictly when computing the element
matrices.


Finding the total number of nodes to be computed:
~~~~~~~~~~~~~~~~~~~~~~~~~~~~~~~~~~~~~~~~~~~~~~~~~

The following formula is to find the total number of computational nodes
(including the GLL points) for a rectangular mesh which have to be
solved for at each time step:

.. math::

   \begin{aligned}
   N_{total} &=& ((n_y \times N_y) - (N_y - 1)) \times (N_x + 1) \nonumber \\ &+& ((n_x - 2) \times N_x) \times (N_y + 1) \nonumber \\ + ((n_x &\times& n_y - 2 (n_y + n_x) + 4))\times (N_x \times N_y)\end{aligned}

where, :math:`n_i` is the number of nodes per element in the along i-th
coordinate and :math:`N_i` is the number of elements along the i-th
coordinate. Therefore, if we have a mesh with :math:`n_x` = :math:`n_y`
= 5 and :math:`N_x` = 20 and :math:`N_y` = 10, then :math:`N_{total}` =
3321.


Lagrange Polynomials
~~~~~~~~~~~~~~~~~~~~

The chosen test functions for the spectral element method are the
Lagrange polynomials. The Lagrange polynomials are interpolation
polynomials between certain points and defined in the following manner.

.. math::

   \label{eq:lagrange}
       \ell^n_i(\xi) = \prod_{\substack{j = 0\\ j \neq i}}^{n+1} \frac{\xi - \xi_j}{\xi_i - \xi_j},

where :math:`\xi_i` are the collocation points, :math:`i` is the number
of the polynomial with respect to collocation points and :math:`n` is
the degree of the polynomial :cite:`Komatitsch1999`. 
I.e., the elaborate expression would look like this:
The SEMâ€™s signature shape functions are the Lagrange Polynomials
:math:`l^{n_l}_\alpha`:

.. math:: 

       \ell _ { \alpha } ^ { n _ { \ell } } ( \xi ) = \frac { \left( \xi - \xi _ { 0 } \right) \cdots \left( \xi - \xi _ { \alpha - 1 } \right) \left( \xi - \xi _ { \alpha + 1 } \right) \cdots \left( \xi - \xi _ { n _ { \ell } } \right) } { \left( \xi _ { \alpha } - \xi _ { 0 } \right) \cdots \left( \xi _ { \alpha } - \xi _ { \alpha - 1 } \right) \left( \xi _ { \alpha } - \xi _ { \alpha + 1 } \right) \cdots \left( \xi _ { \alpha } - \xi _ { n _ { \ell } } \right) }

where :math:`\alpha = 0,...,n_l`, and :math:`n_l` will be 5 to 10 (in
our case).
The implemented algorithm follows this formulation strictly. In multiple
dimensions, the shapefunctions :math:`N`, are defined as the product of
the polynomials in each dimension., i.e.
:math:`N_{kl}(\xi,\eta) = \ell^n_k(\xi)\ell^n_l(\eta).`



Derivative of the Lagrange Polynomials
~~~~~~~~~~~~~~~~~~~~~~~~~~~~~~~~~~~~~~

As seen in the formulation section, the spectral element method also
requires the derivative of the shape functions. The derivative of the
Lagrange polynomials are defined as the original Lagrange polynomial
multiplied by the Legendre polynomial. The Legendre polynomial
:math:`P^n_i` is given by following sum

.. math:: P^n_i(\xi) = \sum_{\substack{j = 0\\ j \neq i}}^{n+1} \frac{1}{\xi - \xi_j},

where :math:`\xi_i` are the collocation points, :math:`i` is the
polynomial number with respect to the collocation point and :math:`n` is
the polynomial degree. Hence, the derivative of the Lagrange polynomial
(Eq. [eq:lagrange]) is given as

.. math:: \frac{d\ell^n_i}{d\xi} = P^n_i(\xi)\ell^n_i(\xi).

The equation becomes more elaborate when writing out all the component:

.. math:: \frac{d\ell^n_i}{d\xi} =  \sum_{\substack{k = 0\\ k \neq i}}^{n+1} \left( \frac{1}{\xi - \xi_k} \prod_{\substack{j = 0\\ j \neq i}}^{n+1} \frac{\xi - \xi_j}{\xi_i - \xi_j} \right)

This cannot be implemented as strictly as the Lagrange polynomial itself
since it would include a division by :math:`0` at :math:`\xi = \xi_k`.
However, a quick look at the denominator in the first term and the
numerator on the second term shows, that we have a cancellation when
:math:`(\xi - \xi_k) =  (\xi - \xi_j)`, or shorter, when :math:`k=j`,
such that

.. math::

   \frac{d\ell^n_i}{d\xi} =  \sum_{\substack{k = 0\\ k \neq i}}^{n+1} \left[ \prod_{\substack{j = 0\\ j \neq i}}^{n+1} \left\{ \begin{array}{ll}
           \frac{1}{\xi_i - \xi_j},  & \text{if } k=j \\
           \frac{\xi - \xi_j}{\xi_i - \xi_j}, & \text{otherwise}
       \end{array} \right. \right].

This is strictly followed in the algorithm.

The Jacobian
~~~~~~~~~~~~

The Jacobian between local and global coordinates can be defined as

.. math:: 

       \frac { \partial \mathbf { x } } { \partial \xi } = \sum _ { a = 1 } ^ { n _ { a } } \frac { \partial N _ { a } } { \partial \xi } \mathbf { x } _ { a }

In practice we use the inverse Jacobian matrix for each node to 
compute the global derivative at its location using 
``src.gll_library.dN_local_2D`` and ``src.gll_library.global_derivative``.
``dN_local_2D()`` computes the local derivative matrix containing derivatives
in each dimension of each shape function and ``global_derivative``, then takes in 
the Jacobian computes its inverse and multiplies it with the local derivative 
matrix to compute the global derivative matrix.

Element and Node Numbering
--------------------------

The method developed here relies on a FEM mesh created by an external
meshing software, which creates a ``.e`` Exodus file. The Exodus file
provides all the necessary information for a mesh: (a) the coordinates
of the nodes defining the control points, (b) connectivity of the
elements, as well as (c) the boundary nodes. This information is used to
create an arbitrary number of interpolation points on each element with
a new set of connectivity and numbers. This ensures that increasing
computational power can be harnessed for higher accuracy. The input mesh
therefore contains only quadrilaterals defined by four nodes (as of now;
will be extended to higher number of nodes in the future). The functions
used to read and redefine the mesh are located within the
``src/mesh_spec.py`` script. The numbering itself is performed using the
following algorithm shown in figure [fig:element\_numbering].

.. figure:: figures/element_fig_edit.pdf
   :alt: Control points of initial mesh vs GLL collocation points

   Example of GLL node and element numbering algorithm using 5x5 GLL
   points and two elements. The numbers in the red, rounded boxes denote
   the element number. The circles and white boxed numbers show the
   control point locations and numbers, respectively. the small crosses
   and numbers show the GLL point locations and numbers, respectively.

In the figure, we show the GLL points in each direction, and also the
GLL points lie on the edges as well as the interior of each element. The
locations of the GLL points contribute to the simplification of the mass
matrix, which becomes diagonal, because of the GLL quadrature used.

The interpolation of the GLL points on the Mesh of quadrilaterals is 
governed by the following equation

.. math:: \mathbf { x } ( \xi , \eta ) = \sum _ { a = 1 } ^ { n _ { a } } N _ { a } ( \xi , \eta ) \mathbf { x } _ { a }.

where :math:`N` are the basis functions, also called the shape function, 
namely, the Lagrange Polynomials. This step is applied within the module and 
function ``src.mesh_spec.mesh_interp2D()``.

Global Matrix Assembly
----------------------


.. figure:: figures/element_fig.pdf
       :alt: Control points of initial mesh vs GLL collocation points

       Same figure as above. Just to demonstrate that the nodes on the
       right edge of element and left edge of element one coincide.

Since the nodes :math:`[1,6,11,16,21]` are on the edge of both elements,
the contributions of both elements have to be considered. To achieve this
a global set of linear equations is set up. The local numbering within the 
element is the same for every element since the collocation points of the 
shape function depend on it. Therefore, there needs to be a mapping from 
local to global coordinates. This transformation is done by 
``src.loc2glob.local2global()``. 

The algorithm works using the following setup.

.. figure:: figures/localglobalnumbering.pdf
       :alt: local2global

       Small two element four GLL points per node setup. (a) shows the 
       local numberig for each element and (b) shows the global set of 
       nodes.

This setup will result in a 6x6 mass and stiffness matrix.

The connectivity setup is then:

.. math:: 

       \begin{equation}
              \text{Connnectivity} = \left[ 
                \begin{array} { c c c c } 
                    { 1 } & { 2 } & { 3 } & { 4 } \\ 
                    { 5 } & { 1 } & { 6 } & { 3 } \\ 
                  \end{array} \right]
       \end{equation}

The element matrices look like this for each stiffness matrix:

.. math::
       \begin{equation}
       \mathbf { K } ^ { e } = \left[ \begin{array} { c c c c } 
              { K _ { 11 } ^ { e } } & { K _ { 12 } ^ { e } } & { K _ { 13 } ^ { e } } & { K _ { 14 } ^ { e } } \\ 
              { K _ { 21 } ^ { e } } & { K _ { 22 } ^ { e } } & { K _ { 23 } ^ { e } } & { K _ { 24 } ^ { e } } \\ 
              { K _ { 31 } ^ { e } } & { K _ { 32 } ^ { e } } & { K _ { 33 } ^ { e } } & { K _ { 34 } ^ { e } } \\ 
              { K _ { 41 } ^ { e } } & { K _ { 42 } ^ { e } } & { K _ { 43 } ^ { e } } & { K _ { 44 } ^ { e } } 
              \end{array} \right]
       \end{equation}

The total range of :math:`e`, which denotes the element number, is :math:`[1,2]`. 
Using the new stiffness matrix we can then assemble the global stiffness matrix.
As an example, consider the term :math:`K^2_{13}`. Since the term is from element 1, 
row 1 of Connnectivity has to be checked where we see that the local nodes 1 and 3 
(i.e., the first and third column) map to the global indices 5 and 6 respectively.
That means, the :math:`K^1_{13}` has to be mapped into the global matrix in row 5
and column 6.

.. math:: 

       \mathbf{ K } _ { global } = \left[ \begin{array} { c c c c c c } 
       { K _ { 11 } ^ { 1 } } + { K _ { 22 } ^ { 2 } } & { K _ { 12 } ^ { 1 } } & { K _ { 13 } ^ { 1 } } + { K _ { 24 } ^ { 2 } } & { K _ { 14 } ^ { 1 } } & { K _ { 21 } ^ { 2 } } & { K _ { 23 } ^ { 2 }} \\ 
       { K _ { 21 } ^ { 1 } } & { K _ { 22 } ^ { 1 } } & { K _ { 23 } ^ { 1 } } & { K _ { 24 } ^ { 1 } } & 0 & 0 \\ 
       { K _ { 31 } ^ { 1 } }+ { K _ { 42 } ^ { 2 } } & { K _ { 32 } ^ { 1 } } & { K _ { 33 } ^ { 1 } } + { K _ { 44 } ^ { 2 } } & { K _ { 34 } ^ { 1 } } & { K _ { 41 } ^ { 2 } } & { K _ { 43 } ^ { 2 } }\\  
       { K _ { 41 } ^ { 1 } } & { K _ { 42 } ^ { 1 } } & { K _ { 43 } ^ { 1 } } & { K _ { 44 } ^ { 1 } } & 0 & 0\\
       { K _ { 12 } ^ { 2 } } & 0 & { K _ { 14 } ^ { 2 } } & 0 & { K _ { 11 } ^ { 2 } } & { K _ { 13 } ^ { 2 } }\\ 
       { K _ { 32 } ^ { 2 } }& 0 & { K _ { 34 } ^ { 2 } } & 0 & { K _ { 31 } ^ { 2 } } & { K _ { 33 } ^ { 2 } }\end{array} \right]

This can be done for both the stiffness and the mass matrix, as well as the 
force vector.

Then, we end up with following system of equations:

.. math:: \mathbf{M} \ddot { \mathbf{u} } + \mathbf{K} \mathbf{u} = \mathbf{f}

However, :math:`\mathbf{u}` is still dependent on time. To solve this a
simple finite difference scheme can be applied or other time marching
methods.



Time Marching
-------------

Timestep is done by ``class`` Tscheme which is written in `src/tscheme.py`. It can solve ODEs
with the following type:

`First order ODEs`


First order ODEs with constant mass matrix :math:`M` and constant stiffness matrix :math:`K`
and time varient force term :math:`F(t)` can be solved. Equation then has the form
:math:`M\dot{X}+KX=F(t)`.


`Second order ODEs`


First order ODEs with constant mass matrix :math:`M` ,
constant absorbing matrix :math:`C`and constant stiffness matrix :math:`K`
and time varient force term :math:`F(t)` can be solved. Equation then has the form
:math:`M\ddot{X}+C\dot{X}+KX=F(t)`. If you are using schemes for first order equations like
`euler_explicit`, `rk4`, the equations will be turned into the following first order ODEs.




.. math:: \begin{pmatrix} I & O \\ O & M \end{pmatrix}\left( \begin{array}{c} \dot { X }  \\ \dot { P }  \end{array} \right) +\begin{pmatrix} O & -I \\ K & C \end{pmatrix}\left( \begin{array}{c} X \\ P \end{array} \right) =\left( \begin{array}{c} O \\ F \end{array} \right)


If you are using newmark, then the absorbing matrix :math:`C` has to be zero, please set `C=None` when
you use the solver.

^^^^^^^^^^^^^^^^^^^^^^^^^^^^^^^^^^^^^^

`Usage`

First Specify the following arguments

- ``M:`` mass matrix, ``numpy`` [N]x[N] array

- ``C:`` absorbing matrix, default None

- ``K:`` stiffness matrix, ``numpy`` [N]x[N] array

- ``f:`` force term f(t), given t return the force vector of type ``numpy`` [N] array.

- ``t:`` time vector for stepping, t[0] should be the start time

- ``outdir:`` result output directory

- ``gamma:`` parameter for Newmark scheme, default 0.5

- ``solver:`` name of the main solver, default euler_explicit

- ``solver2:`` solver for the first few steps of the multistep method,
                    default rk4

- ``interval:`` interval for output the result, should be an integer,
                     default 1


Then create a `Tscheme` object by


``tstep=tscheme.Tscheme(M=M,K=K,f=f,t=t,outdir=outdir,solver=solver)``

Then run the solver by

``tstep.process()``



^^^^^^^^^^^^^^^^^^^^^^^^^^^^^^^^^^^^^^

`Details of implementation`

For all the kinds of solvers, the Tscheme will automatically turn the equations into
standard form. That is using transformation :math:`U=MX` to make mass matrix :math:`M`
unit. The `src/tsolver.py` contains all the solver thant can solve equations with
unit mass matrix.

For first order solvers, like `euler_explicit`, `rk4`, the solvers in `src/tsolver.py` can
solve equations with form :math:`\dot{U}=F(U,t)`, the equation we are going to solve is
:math:`\dot{U}+K{ M }^{ -1 }U=F(t)`, here our :math:`F(U,t)=F(t)-K{ M }^{ -1 }U`.

For second order solvers newmark, the algorithm is as follows:

+----+--------------------------------------------------------+
| **Algorithm 1**                                             |
+====+========================================================+
| 1: | **Procedure** :math:`\text{NEWMARK}(U_n,V_n,A_n,dt,F)` |
+----+--------------------------------------------------------+
| 2: | :math:`U_{n+1}=U_n+V_ndt+0.5A_ndt^2`                   |
+----+--------------------------------------------------------+
| 3: | :math:`A_{n+1}=F_{n+1}-KM^{-1}U_{n+1}`                 |
+----+--------------------------------------------------------+
| 4: | :math:`V_{n+1}=(1-\gamma)A_{n}dt+\gamma A_{n+1}dt`     |
+----+--------------------------------------------------------+
| 5: | **return** :math:`U_{n+1},V_{n+1},A_{n+1}`             |
+----+--------------------------------------------------------+

After solving :math:`U`, use transformation :math:`X={M}^{-1}U` to get :math:`X`





